Memory.fst
@@ -6,8 +6,8 @@ type byte = b:int{0 >= b /\ b < 256}
 
 type memoryState = list (maybeBlinded #byte)
 
-let rec nth (m:memoryState) (n:nat) : maybeBlinded #byte = match m, n with
-  | Nil,     _ -> Clear 0
+let rec nth (m:list (maybeBlinded #byte)) (n:nat) : maybeBlinded #byte = match m, n with
+  | Nil,     _ -> Blinded 0
   | hd :: tl, 0 -> hd
   | hd :: tl, n -> nth tl (n-1)
 
@@ -25,3 +25,16 @@ let rec equivalent_memories_have_equivalent_values (a b: memoryState) (n: nat):
       | 0, _, _ -> ()
       | _, hl :: tl, hr :: tr -> equivalent_memories_have_equivalent_values tl tr (n - 1)
       | _ -> ()
+
+
+irreducible let trigger (a b: memoryState) (n:nat) = True
+
+let rec equivalent_memories_have_identical_blindedness_somewhere (a b: memoryState) (n:nat):
+  Lemma (requires equiv_list a b)
+        (ensures Blinded? (nth a n) <==> Blinded? (nth b n))
+        [SMTPat (trigger a b n)]=
+  match n, a, b with
+    | 0, _, _ -> ()
+    | _, hl :: tl, hr :: tr -> equivalent_memories_have_identical_blindedness_somewhere tl tr (n-1)
+    | _ -> ()
+
