Value.fst
@@ -18,6 +18,11 @@ let equiv lhs rhs
       | _ -> false
 
 
+let equal_values_are_equivalent (t:eqtype) (lhs rhs:maybeBlinded #t):
+  Lemma (requires lhs = rhs)
+        (ensures equiv lhs rhs) =
+  ()
+
 let redact (#t:Type) (x: maybeBlinded #t) (d:t): maybeBlinded #t =
     match x with
     | Clear   v -> Clear v
@@ -29,7 +34,6 @@ let _ = assert(forall (t:eqtype) (x y d: t). redact (Blinded x) d == redact (Bli
 let values_are_equivalent_to_their_redaction (t:eqtype) (x:maybeBlinded #t) (d:t):
     Lemma (ensures equiv x (redact x d))
     = ()
-
 
 let equivalent_values_have_equal_redactions (t:eqtype) (x y:maybeBlinded #t) (d:t):
     Lemma (ensures equiv x y <==> redact x d = redact y d)
@@ -57,10 +61,31 @@ let rec equiv_list (lhs:list maybeBlinded) (rhs: list maybeBlinded)
        | Cons _ _, Nil      -> false
        | lh :: lt,  rh :: rt  -> (equiv lh rh) /\ (equiv_list lt rt)
 
-let rec redact_list (#t:eqtype) (pre:list (maybeBlinded #t)) (d:t): list (maybeBlinded #t)
+let rec redact_list (#t:eqtype) (pre:list (maybeBlinded #t)) (d:t): r:(list (maybeBlinded #t)){FStar.List.length r = FStar.List.length pre}
     = match pre with
       | Nil         -> Nil
       | head :: tail -> (redact head d) :: (redact_list tail d)
+
+let rec equivalent_lists_have_equal_lengths (#t:eqtype) (l1 l2:list (maybeBlinded #t))
+  : Lemma (requires equiv_list l1 l2)
+          (ensures FStar.List.length l1 = FStar.List.length l2)
+  = match l1, l2 with
+    | h1 :: t1, h2 :: t2 -> equivalent_lists_have_equal_lengths t1 t2
+    | _ -> ()
+
+let rec redaction_preserves_length (t:eqtype) (x:list(maybeBlinded #t)) (d:t)
+  : Lemma (ensures FStar.List.length x = FStar.List.length (redact_list x d))
+  = match x with
+    | Nil -> ()
+    | hd :: tl -> redaction_preserves_length t tl d
+
+let rec equal_lists_are_equivalent (t:eqtype) (lhs rhs:list(maybeBlinded #t)):
+    Lemma (requires lhs = rhs)
+          (ensures equiv_list lhs rhs) =
+    match lhs, rhs with
+      | Nil, Nil -> ()
+      | hl :: tl, hr :: tr -> (equal_values_are_equivalent t hl hr;
+                            equal_lists_are_equivalent t tl tr)
 
 let rec lists_are_equivalent_to_their_redaction (t:eqtype) (x: list(maybeBlinded #t)) (d:t)
     : Lemma (ensures equiv_list x (redact_list x d))
@@ -91,3 +116,30 @@ let rec list_equivalence_is_transitive (t:eqtype) (lhs mid rhs: list(maybeBlinde
     = match lhs, mid, rhs  with
       | hl :: tl, hm :: tm, hr :: tr -> list_equivalence_is_transitive t tl tm tr
       | _ -> ()
+
+let rec nth (#t:eqtype) (m:list (maybeBlinded #t)) (n:nat{n < FStar.List.length m}): maybeBlinded #t = match m, n with
+    | hd :: tl, 0 -> hd
+    | hd :: tl, n -> nth tl (n-1)
+
+
+let rec equivalent_lists_have_equivalent_values (t:eqtype) (a b: list (maybeBlinded #t)) (n: nat{n < FStar.List.length a && n < FStar.List.length b}):
+    Lemma (requires equiv_list a b)
+          (ensures equiv (nth a n) (nth b n))
+    = match n, a, b  with
+      | 0, _, _ -> ()
+      | _, hl :: tl, hr :: tr -> equivalent_lists_have_equivalent_values _ tl tr (n - 1)
+      | _ -> ()
+
+let rec all_values_are_blinded (t:eqtype) (l: list (maybeBlinded #t)) =
+  match l with
+    | hd :: tl -> if Clear? hd then false else all_values_are_blinded t tl
+    | _ -> true
+
+let rec lists_of_blinded_values_of_equal_length_are_equivalent (t:eqtype) (a b: list (maybeBlinded #t)):
+  Lemma (requires (FStar.List.length a = FStar.List.length b) /\ (all_values_are_blinded t a) /\ (all_values_are_blinded t b))
+        (ensures equiv_list a b) =
+  match a, b with
+    | h1 :: t1, h2 :: t2 -> (
+         lists_of_blinded_values_of_equal_length_are_equivalent t t1 t2
+      )
+    | _ -> ()
